AddOns/AngelicVerifierNull/test/regression/doubleFree.bpl
@@ -1,29 +1,23 @@
 procedure {:entrypoint} main() {
  var p : int;
  call p := unknown();
- //assume(~valid[p]);
  call foo(p);
 }
 
 procedure foo(p: int)
 {
-  assert ~valid[p];
-  call ~free(p);
-  assert ~valid[p];
-  call ~free(p);
+  assert valid[p];
+  call free(p);
+  assert valid[p];
+  call free(p);
   return;
 }
 
-
-//procedure {:~free} ~free(a: int);
-// modifies ~valid;
-// free ensures ~valid == old(~valid)[a := false];
-
-procedure {:~free} ~free(a: int) {
- ~valid[a] := false;
+procedure {:free} free(a: int) {
+ valid[a] := false;
 }
 
-var ~valid: [int]bool;
+var {:propertyMap} valid: [int]bool;
 
 const {:allocated} NULL : int;
 
